x^2-2x-3=0
$$
$$
x^2-3x+x-3=0
$$
$$
x(x-3)+1(x-3)=0
$$
$$
(x+1)(x-3)
$$
$$
x=-1
$$
$$
x=3
$$
$$
P=\{-1,3\}
$$
$$
Q=\{1,5,10,15,20,...\}
$$
$$
x^2=64
$$
$$
S=\{-8,8\}
$$
28=10
19=10
55=10
A={28,19,55,73,64,82,91,37,}
B={28,15,19,55,73,64,82,91,37,}
A$\neq$B
n(A)={8}

B={E,N,G,I,R,T,....}

A={a:a is a multiple of 13; 1<a<$\infty$}
B={b:b is a prime number; 1<b<100}
C={c:c is a natural number; 1<=1/c<$\infty$}
$$
C=\{c:\}
$$
$$
\begin{align}
x^2-3x+2\\
x^2-2x-x+2\\
x(x-2)-1(x-2)\\
(x-2)(x-1)
\end{align}
$$
$$
C=\{2,1\}
$$
# Subset
A={1,2,3,4,5}
B={1,2,3,4,5}
C={1,2,3}
A$\subseteq$ B 
B$\not\subseteq$C
A$\not\subseteq$C
C$\subseteq$B

## Proper Subset
If A and B are sets and every element of A is also an element of B.
A={1,2,3,4,5}
B={1,2,3,4,5}
C={1,2,3}
n(p(c))=

A$\not\subset$B
C$\subset$A = C$\subseteq$A

A={3,9,12}
B={2,4,9,12}

A$\not\subseteq$B
A$\subset$B


## Difference of Sets
A={1,2,3,4}
B={3,4,5,7}

A-B={1,2}
B-A={5,7}

A-B$\neq$ B-A

## Laws of Algebra

### Identity Laws
A={1,2,3,4}
B={3,4,5,7}

$A \cup \varnothing = A$ 
$A \cap u = A$ 

> [!note]
> $A \cup u = u$
> $A \cap \varnothing = \varnothing$ 
### Idempotent Laws
$$
A\cup A = A
$$
$$
A \cap A = A
$$
### Commutative Laws
$$
A\cup B= B\cup A
$$
$$
A\cap B=B\cap A
$$
$$
A={1,2,3,4}
B={1,2,3,4,6,7,8,9}
C={15,19,21}

B-A = {6,7,8,9}
A-B = {$\varnothing$}






A $\cup$ C = {1,2,3,4,15,19,21} # Union
A $\cap$ B = {1,2,3,4} # Intersection


A $\cap$ C = {$\varnothing$} # Disjoint sets



u-A={6,7,8,9}=A complement
A $\cup$ B = {1,2,3,4,5,7}
B $\cup$ A = {5,7,1,2,3,4}


X={{a},{b},{c},{d},{a,b},{b,c},{a,c},{$\varnothing$}}

Y={{1},{2},{3},{4},{1,2},{1,3},{1,4},{2,3},{2,2},{2,4},{3,3},{3,4},{4,4},{1,2,3},{},{$\varnothing$}}



$$
a^2+2ab+b^2
$$
$$
49y^2+70y+( )
$$
$$
(7y)^2+7\times2\times 5 \times y+(25)
$$
$$
16q^2-24q+()
$$
$$
(4q)^2-2(12q)+()
$$
$$
(4q)^2-2(4\times3\times q) + 9
$$
$$
16- () + 121x^2y^2
$$
$$
121x^2y^2-()+16
$$







$$
(4q)^2-4\times2\times 3 + 9
$$

$$
a^2+2ab+b^2
$$
$$
a^2-2ab+b^2
$$
---

$$
(4q)^2=a^2
$$
$$
-2ab=-24q
$$
$$
b^2=?
$$
$$
4q=a
$$
$$
-2\times 4q \times b = 24q
$$
$$
b=3
$$
---
$$
a^2=49y^2
$$
$$
a=7y
$$
$$
70y=2ab
$$
$$
70y=2 \times 7y \times b
$$
$$
70y=14yb
$$
$$
\frac{70y}{14y}=b
$$
$$
b=5
$$

---
$$
a^2=9x^2
$$
$$
a=3x
$$
$$
b = 5y
$$

---
$$
121x^2y^2-()+16
$$
$$
a=11xy
$$
$$
b=4
$$
---

$$
x^2-13x-30
$$
$$
x^2-15x+2x-30
$$


---
$$
2a^2-2\sqrt{2}a+()
$$
$$
a=\sqrt{2}a
$$
$$
2ab=2 \times \sqrt{2}a \times b
$$
---

$$
x^2-13x-30
$$
$$
x^2-15x+2x-30
$$
$$
x(x-15)+2(x-15)
$$
$$
(x+2)(x-15)
$$
---
$$
x^2-2x-24
$$
$$
x^2-6x+4x-24
$$
$$
x(x-6)+4(x-6)
$$
---
$$
x^2+3x-18
$$
$$
x^2+6x-3x-18
$$
$$
x(x+6)-3(x+6)
$$
$$
(x+6)(x-3)
$$
---
$$
y^6+3y^3-108
$$
$$
y^6+12y^3-9y^3-108
$$
$$
y^3(y^3+12)-9(y^3+12)
$$
---
$$
y^2-8y-20
$$
$$
y^2-10y+2y-20
$$
$$
y(y-10)+2(y-10)
$$
---
$$
m^2-19m+48
$$
$$
m^2-16m-3m+48
$$
$$
m(m-16)-3(m-16)
$$
---

$$
21x^2+23xy+6y^2
$$
$$
21x^2+18xy+7xy+6y^2
$$
$$
3x(7x+6y)+y(7x+6y)
$$
---
$$
15x^2-31xy+14y^2
$$
---
$$
2^4a^4-3^4b^4
$$
$$
((2a)^2-(3b)^2)^2
$$
$$
((2a)^2+(3b)^2)((2a)^2-(3b)^2)
$$
$$
((2a)^2+(3b)^2)((2a)+(3b))((2a)-(3b))
$$

---
$$
x^2-y^2=(x+y)(x-y)
$$
$$
(x+2)^2-x^2
$$
$$
((x+2)-x)((x+2)+x)
$$
$$
2(2x+2)
$$
$$
4(x+1)
$$
---
$$
(a+b-c)^2-(a-b+c)^2
$$
$$
((a+b-c)+(a-b+c))((a+b-c)-(a+b-c))
$$
---
$$
(x+y)^2=(x+y)(x+y)
$$
$$
(x-y)^2=(x-y)(x-y)
$$
---
$$
625x^8-81
$$
$$
5^4x^8-9^2
$$
$$
(5^2x^4)^2-9^2
$$
$$
((5^2x^4)-9)((5^2x^4)+9)
$$
$$
((5x^2)^2-3^2)((5^2x^4)+3^2)
$$
$$
((5x^2)-3)((5x^2)+3)((5^2x^4)+9)
$$

