Find the set of $x$ such that $(4x^2-9)(x^2+4x+4)\leq 0$ where $x \in \mathbb{R}$.

$$
\begin{align}
(4x^2-9)(x^2+4x+4)\leq 0 \\ \\
(2x-3)(2x+3)(x+2)(x+2)\\ \\
(2x-3)\leq0\\ \\
(2x+3)\leq0\\ \\
(x+2)\leq0
\end{align}
$$
$$
\begin{align}
x\leq\frac{3}{2}\\ \\
x \leq -\frac{3}{2}\\ \\
x \leq -2
\end{align}
$$

If $x= \frac{3}{2}$;

$$
\begin{align}
(4x^2-9)(x^2+4x+4)\leq 0 \\ \\
(2x-3)(2x+3)(x+2)(x+2) \leq 0 \\ \\
(2\frac{3}{2}-3)(2\frac{3}{2}+3)(\frac{3}{2}+2)(\frac{3}{2}+2) \leq 0\\ \\
(0)(6)(3.5)(3.5)\leq0 \\ \\
0 \leq0
\end{align}
$$
If $x=-\frac{3}{2}$;
$$
\begin{align}
(4x^2-9)(x^2+4x+4)\leq 0 \\ \\
(2x-3)(2x+3)(x+2)(x+2) \leq 0 \\ \\
(2\times-(\frac{3}{2})-3)(2\times-(\frac{3}{2})+3)(-(\frac{3}{2})+2)(-(\frac{3}{2})+2) \leq 0\\ \\
(-6)(0)(0.5)(0.5)\leq0 \\ \\
0 \leq 0
\end{align}
$$
If $x=-2$;
$$
\begin{align}
(4x^2-9)(x^2+4x+4)\leq 0 \\ \\
(2x-3)(2x+3)(x+2)(x+2) \leq 0 \\ \\
(2(-2)-3)(2(-2)+3)((-2)+2)((-2)+2) \leq 0 \\ \\
(12)(-12)(0)(0)\leq0\\ \\
0 \leq 0
\end{align}
$$
Since these three points prove to be true, we can find different points and validate the planes in the given space.

If $x=-3$;
$$
\begin{align}
(4x^2-9)(x^2+4x+4)\leq 0 \\ \\
(2x-3)(2x+3)(x+2)(x+2) \leq 0 \\ \\
(2(-3)-3)(2(-3)+3)(-3+2)(-3+2)\leq 0 \\ \\
(-9)(-3)(-1)(-1)\leq0 \\ \\
27 \nleq 0
\end{align}
$$

Therefore this claims that the given space between $-2<x$ is not valid.

If $x=-1\frac{3}{4}$;
$$
\begin{align}
(4x^2-9)(x^2+4x+4)\leq 0 \\ \\
(2x-3)(2x+3)(x+2)(x+2) \leq 0 \\ \\
(2(-1\frac{3}{4})-3)(2(-1\frac{3}{4})+3)(-(-1\frac{3}{4})+2)(-(-1\frac{3}{4})+2)\leq 0 \\ \\
(-6.5)(-0.5)(1.75+2)(1.75+2) \\ \\
45.70\nleq 0
\end{align}
$$

Therefore this claims that the given space between $-1\frac{3}{4}<x$ is not valid.

If $x=0$;

$$
\begin{align}
(4x^2-9)(x^2+4x+4)\leq 0 \\ \\
(2x-3)(2x+3)(x+2)(x+2) \leq 0 \\ \\
(2(0)-3)(2(0)+3)(0+2)(0+2) \leq 0 \\ \\
(-3)(3)(2)(2)\leq0 \\ \\
-36 \leq0
\end{align}
$$

Therefore this claims that the given space between $-\frac{3}{2}$ and $\frac{3}{2}$ is  valid.

If $x=1\frac{3}{4}$;
$$
\begin{align}
(4x^2-9)(x^2+4x+4)\leq 0 \\ \\
(2x-3)(2x+3)(x+2)(x+2) \leq 0 \\ \\
(2(1\frac{3}{4})-3)(2(1\frac{3}{4})+3)(-(1\frac{3}{4})+2)(-(1\frac{3}{4})+2)\leq 0 \\ \\
(0.5)(6.5)(0.25)(0.25)\leq 0 \\ \\
(0.20)\nleq0
\end{align}
$$
![[Pasted image 20231015211113.png]]

Finally we can conclude that;
$$
x=  \Biggl[-\frac{3}{4},\frac{3}{4} \Biggl],\{-2\}
$$
